Fp/Tactics/Simps.lean
@@ -19,6 +19,7 @@ theorem decide_eq_bool {p} [Decidable p] {b : Bool} (h : p = b)
 -- | TODO: upstream
 attribute [bv_normalize] BitVec.cons
 
+
 -- | TODO: upstream
 open Lean Meta Simp in
 dsimproc [seval, simp, bv_normalize] reduceLog2 (Nat.log2 _) :=
